\documentclass[en, normal, 11pt, black]{elegantnote}

\usepackage{tcolorbox}
\tcbuselibrary{breakable}
\usepackage{amsfonts}
\usepackage{newtxtext}
\usepackage{ulem}
\usepackage{amssymb}

\newenvironment{exercise}[1]{\begin{tcolorbox}[colback=black!15, colframe=black!80, breakable, title=#1]}{\end{tcolorbox}}

\renewenvironment{proof}{\begin{tcolorbox}[colback=white, colframe=black!50, breakable, title=Proof. ]\setlength{\parskip}{0.8em}}{\\\rightline{$\square$}\end{tcolorbox}}

\newenvironment{solution}{\begin{tcolorbox}[colback=white, colframe=black!50, breakable, title=Solution. ]\setlength{\parskip}{0.8em}}{\end{tcolorbox}}

\newcommand{\pder}{\partial\,}

\newcommand{\der}{\,\mathbf{d}}

\title{\textsc{Probability: Problem Set 2}}
\author{\textsc{Zehao Wang}}
\date{\today}

% \vspace{-30pt}

\begin{document}
\maketitle
    \begin{exercise}{1.4.1}
        Show that if $f\geqslant0$ and $\int f\der \mu=0$, the $f=0$ a.e. 
    \end{exercise}

    \begin{proof}
        We need to prove $\mu\left(\left\{x:f(x)>0\right\}\right)=0$. And let $A_\varepsilon=\left\{x:f(x)>\varepsilon\right\}$. So, when $\varepsilon\to0$, $A_\varepsilon\to A_0$. 
        And from the definition of measure, we can know: 
        \begin{align*}
            0\leqslant\varepsilon\mu(A_\varepsilon)=\int_{A_\varepsilon}\varepsilon\der\mu\leqslant\int f\der\mu=0, 
        \end{align*}
        So, $\mu(A_\varepsilon)=0$, and considering the arbitrary of $\varepsilon$, we can know that: 
        \[\mu(A_0)=\lim_{\varepsilon\to0}\mu(A_\varepsilon)=0. \]\vspace{-30pt}
    \end{proof}

    %%%%%%%%%%%%%%%%%%%%%%%%%%%%%%%%%%%%%%

    \begin{exercise}{1.4.2}
        Let $f \geq 0$ and $E_{n, m}=\left\{x: m / 2^{n} \leqslant f(x)<(m+1) / 2^{n}\right\}$. Show that as $n \uparrow \infty$, 
        \[
            \sum_{m=1}^{\infty} \frac{m}{2^{n}} \mu\left(E_{n, m}\right) \uparrow \int f \der \mu. 
        \]
    \end{exercise}

    \begin{proof}
        Let $g=\sum_{m=1}^\infty\frac{m}{2^n}\mathbf{1}_{E_{n,m}}$, $\forall\,x\in E_{n,m}$, $\frac{m}{2^n}<f(x)$. So, we have 
        \[
            \sum_{m=1}^\infty\frac{m}{2^n}\mu(E_{n,m})=\int g\der \mu\leqslant\int f\der \mu. 
        \]
        Hence as $n\to\infty$, $\sup \sum_{m=1}^\infty\frac{m}{2^n}\mu(E_{n,m})\leqslant \int f\der \mu$. 

        For the other inequation, 
        \[
            g+\sum_{m=1}^\infty \frac{1}{2^n}\mathbf{1}_{E_{n,m}}\geqslant f\mathbf{1}_{E_{n,m}}
        \]
        \[
            \frac{1}{2^n}\sum_{m=1}^\infty\mu(E_{n,m})+\sum_{m=1}^\infty\frac{m}{2^n}\mu(E_{n,m})\geqslant\int f\der\mu, 
        \]
        As $n\to 0$, we can write above inequation as: 
        \[
            \sum_{m=1}^\infty\frac{m}{2^n}\mu(E_{n,m})\geqslant\int f\der\mu, 
        \]
        \[
            \inf \sum_{m=1}^\infty\frac{m}{2^n}\mu(E_{n,m})\geqslant\int f\der\mu\geqslant\sup \sum_{m=1}^\infty\frac{m}{2^n}\mu(E_{n,m}). 
        \]
        So, $\sum_{m=1}^{\infty} \frac{m}{2^{n}} \mu\left(E_{n, m}\right) \uparrow \int f \der \mu$. 
    \end{proof}

    %%%%%%%%%%%%%%%%%%%%%%%%%%%%%%%%%%%%%%

    % \begin{exercise}{A.2.1}
    %     Let $B$ be the nonmeasurable set constructed in Theorem A.2.4. 
        
    %     (i) Let $B_{q}=$ $q+^{\prime} B$ and show that if $D_{q} \subset B_{q}$ is measurable, then $\lambda\left(D_{q}\right)=0$. 
        
    %     (ii) Use (i) to conclude that if $A \subset \mathbf{R}$ has $\lambda(A)>0$, there is a nonmeasurable $S \subset A$. 
    % \end{exercise}

    \begin{exercise}{1.4.3}
        Let $g$ be an integrable function on $\mathbb{R}$ and $\varepsilon>0$. 
        
        (i), Use the definition of the integral to conclude there is a simple function 
        \[
            \varphi=\sum_{k} b_{k} \mathbf{1}_{A_{k}},\,\text{with}\int|g-\varphi| \der x<\varepsilon. 
        \]
        
        (ii), Use Exercise A.2.1 to approximate the $A_{k}$ by finite unions of intervals to get a step function 
        \[
            q=\sum_{j=1}^{k} c_{j} \mathbf{1}_{\left(a_{j-1}, a_{j}\right)}
        \]
        with $a_{0}<a_{1}<\cdots<a_{k}$, so that $\int|\varphi-q|<\varepsilon$. 
        
        (iii), Round the corners of $q$ to get a continuous function $r$ so that $\int|q-r| \der x<\varepsilon$. 

        % \textcolor{blue}{\emph{I found something strange, the description of the fourth question seems to be the solution to the third question. }}

        (iv), To make a continuous function replace each $c_{j} \mathbf{1}_{\left(a_{j-1}, a_{j}\right)}$ by a function that is $0$ on $\left(a_{j-1}, a_{j}\right)^{c}$, $c_{j}$ on $\left[a_{j-1}+\delta-j, a_{j}-\delta_{j}\right]$, and linear otherwise. If the $\delta_{j}$ are small enough and we let $r(x)=\sum_{j=1}^{k} r_{j}(x)$, then
        \[
            \int|q(x)-r(x)| \der \mu=\sum_{j=1}^{k} \delta_{j} c_{j}<\varepsilon. 
        \]
    \end{exercise}

    \begin{solution}
        {\large\bf(i)}, From exercise 1.4.2, we can know that if $g\geqslant0$, then 
        \[
            \sum_{m=1}^{\infty} \frac{m}{2^{n}} \mu\left(E_{n, m}\right) \uparrow \int f \der \mu. 
        \]
        Because $g=g^+-g^-$, let 
        \[
            \varphi_1=\sum_{m=1}^\infty\frac{m}{2^n}\mathbf{1}_{E_{n,m}^{g^+}},\ \varphi_2=\sum_{m=1}^\infty\frac{m}{2^n}\mathbf{1}_{E_{n,m}^{g^-}}, 
        \]
        So, we can know that 
        \[\int g^+\der\mu-\int \varphi_1\der\mu=\int|g^+-\varphi_1|\der\mu\leqslant\frac{\varepsilon}{2}, \]
        \[\int g^-\der\mu-\int \varphi_2\der\mu=\int|g^--\varphi_2|\der\mu\leqslant\frac{\varepsilon}{2}, \]
        Hence, we have: 
        \begin{align*}
            \int |g-(\varphi_1-\varphi_2)|\der \mu&=\int |g^+-g^--(\varphi_1-\varphi_2)|\der \mu\\
            &\leqslant\int|g^+-\varphi_1|\der \mu + \int |g^--\varphi_2|\der \mu\\
            &\leqslant\varepsilon. 
        \end{align*}
        {\large\bf(ii)}, \emph{I had a discussion with a few other students, but I still couldn't figure out the relationship between this problem and Exercise A.2.1. }
        
        Knowing that $E_{n,m}$ is disjoint, we can pick $\{A_k\}$ so that $\mu(A_m-E_{n,m})\leqslant\frac{2^n\varepsilon}{k^2}$. And let $q=\sum_{m=1}^k\frac{m}{2^n}\mathbf{1}_{A_m}$then we can get 
        \[\int|\varphi-q|\der\mu\leqslant\sum_{m=1}^k\frac{m}{2^n}\mu(A_m-E_{n,m})\leqslant\varepsilon. \]

        {\large\bf(iii)}, \textcolor{blue}{\emph{I found something strange, the description of the fourth question seems to be the solution to the third question. }}
    \end{solution}
    
    %%%%%%%%%%%%%%%%%%%%%%%%%%%%%%%%%%%%%%

    \begin{exercise}{1.4.4}
        Prove the Riemann-Lebesgue lemma. If $g$ is integrable, then 
        \[
            \lim _{n \rightarrow \infty} \int g(x) \cos(nx) \der x=0. 
        \]
        Hint: If $g$ is a step function, this is easy. Now use the previous exercise. 
    \end{exercise}

    \begin{proof}
        From Exercose 1.4.3, we know that $g$ can be approximated by the step function, i.e. $g(x)=\sum_{i=1}^\infty m_i \mathbf{1}_{(a_i, b_i)}(x)$, and since $g$ is integrable, $\int g(x)\der x=\sum_{i=1}^\infty m_i\mu((a_i,b_i))<\infty$, then 
        \[
            \int g(x) \cos (n x )\der x=\sum_{i=1}^\infty m_i \int_{a_i}^{b_i} \cos (n x) \der x\leqslant\frac{1}{n}\sum_{i=1}^\infty m_i\mu((a_i,b_i)), 
        \]
        So, $n\to \infty$, $\int g(x) \cos (n x )\der x\rightarrow 0$. 
    \end{proof}

    %%%%%%%%%%%%%%%%%%%%%%%%%%%%%%%%%%%%%%

    \begin{exercise}{1.5.2}
        Show that if $\mu$ is a probability measure, then
        \[
            \|f\|_{\infty}=\lim_{p\to\infty}\|f\|_p. 
        \]
    \end{exercise}

    \begin{proof}
        For some $N$, if $\mu(\{x:f(x)\geqslant N\})=0$, then
        \[
            \left(\int |f|^p\der\mu\right)^{\frac{1}{p}}\leqslant N, 
        \]
        Then, 
        \[
            \lim\sup_{p\to\infty}\|f\|_p\leqslant N. 
        \]
        For some $M$, if $\mu(\{x:f(x)\geqslant M\})=m>0$, then
        \[
            \left(\int|f|^p\der \mu\right)^{\frac{1}{p}}\geqslant\sqrt[p]{m}M, 
        \]
        Then 
        \[
            \lim\inf_{p\to \infty}\|f\|_p\geqslant M. 
        \]
        And because $\|f\|_\infty=\sup\{|f(x)|\}$, let $m\to0$, we can get that $\sup\{|f(|x|)\}=M=N=\lim_{p\to\infty}\|f\|_p$. 
    \end{proof}

    %%%%%%%%%%%%%%%%%%%%%%%%%%%%%%%%%%%%%%

    \begin{exercise}{1.5.7}
        Let $f\geqslant0$. 
        
        (i) Show that
        \[
            \int f\wedge n\der\mu\uparrow\int f\der\mu,\,\text{as}\,n\to\infty. 
        \]
        (ii) Use (i) to conclude that if $g$ is integrable and $\varepsilon>0$, then we can pick $\delta > 0$ so that $\mu(A) < \delta$ implies
        \[
            \int_A|g|\der\mu<\varepsilon. 
        \]
    \end{exercise}

    \begin{proof}
        (i), We can know that $f\wedge n\leqslant f\wedge (n+1)$, and $\lim_{n\to \infty}(f\wedge n)=f$. So, \[\int f\wedge n\der\mu\uparrow\int f\der\mu. \]
        (ii), Let $f=|g|$, then, $|g|\geqslant (|g|\wedge n)$, for any $n\in\mathbb{Z}^+$. Because $\int |g|\wedge n\der\mu\uparrow\int |g|\der\mu$, there exist $n$, such that
        \[
            \int_A |g|\der\mu-\int_A |g|\wedge n\der\mu\leqslant \frac{\varepsilon}{2}. 
        \]
        Pick $\delta=\frac{\varepsilon}{2n}$, then we have
        \begin{align*}
            \int_A|g|\der\mu&\leqslant\int_A|g|\der\mu-\int_A |g|\wedge n\der\mu+\int_A |g|\wedge n\der\mu\\
            &\leqslant\frac{\varepsilon}{2}+\mu(A)n<\varepsilon. 
        \end{align*}
        \vspace{-30pt}
    \end{proof}

    %%%%%%%%%%%%%%%%%%%%%%%%%%%%%%%%%%%%%%

    \begin{exercise}{1.6.1}
        Suppose $\varphi$ is strictly convex, i.e., $>$ holds for $\lambda \in(0,1)$. Show that, under the assumptions of Theorem 1.6.2, $\varphi(E X)=E \varphi(X)$ implies $X=E X$ a.s. 
    \end{exercise}

    \begin{proof}
        Because $\varphi$ is strictly convex, there exist $c$, such that when $x\not=x_0$, 
        \[
            \varphi(x)-\varphi(x_0)>c(x-x_0), 
        \]
        Let $x_0=EX$, we can get that 
        \[
            \varphi(x)>c(x-EX)+\varphi(EX), 
        \]
        From Jensen's inequality, we know that if $\varphi(EX)=E\varphi(X)$, then $E(x-EX)=0$, i.e. $P(X=EX)=1$, $X=EX$, a.e. 
    \end{proof}

    %%%%%%%%%%%%%%%%%%%%%%%%%%%%%%%%%%%%%%

    \begin{exercise}{1.6.2}
        Suppose $\varphi: \mathbb{R}^{n} \rightarrow \mathbb{R}$ is convex. Imitate the proof of Theorem $1.5.1$ to show
        \[
            E \varphi\left(X_{1}, \ldots, X_{n}\right) \geq \varphi\left(E X_{1}, \ldots, E X_{n}\right). 
        \]
        provided $E\left|\varphi\left(X_{1}, \ldots, X_{n}\right)\right|<\infty$ and $E\left|X_{i}\right|<\infty$ for all $i$. 
    \end{exercise}

    \begin{proof}
        Because $\varphi$ is convex, let $X$ denote $(X_1, \cdots, X_n)$ and we can get a linear function $l(X)=\varphi(E(X))+\sum_{i=1}^na_i(X_i-E(X_i))$, which satisfy for some $c=E(X)$, $l(c)=\varphi(c)$, and for other $x\not=c$, $\varphi(X)>l(X)$, 
        \[
            E(\varphi(X))\geqslant E\left(l(X)\right)=\varphi(E(X))+\sum_{i=1}^na_i(E(X_i)-E(X_i))=\varphi(E(X)). 
        \]
        \vspace{-30pt}
    \end{proof}

    %%%%%%%%%%%%%%%%%%%%%%%%%%%%%%%%%%%%%%

    \begin{exercise}{1.6.3. Chebyshev's inequality is and is not sharp.}        
        (i) Show that Theorem $1.6.4$ is sharp by showing that if $0<b \leq a$ are fixed there is an $X$ with $E X^{2}=b^{2}$ for which $P(|X| \geq a)=b^{2} / a^{2}$. 
        
        (ii) Show that Theorem 1.6.4 is not sharp by showing that if $X$ has $0<E X^{2}<\infty$, then
        \[
            \lim _{a \rightarrow \infty} a^{2} P(|X| \geq a) / E X^{2}=0. 
        \]
    \end{exercise}

    \begin{proof}
        (i), Let $P(|X|=a)=P(X=a)+P(X=-a)=\frac{b^2}{a^2}$, and $P(X=0)=1-P(|X|=a)$. And $E(X)=0$, $E(X^2)=Var(X)=b^2$. If $i_{A}=\inf\,\{\varphi(y): y \in A\}$, then we need to prove that
        \[
            i_{A}\,P(X \in A) \leq E(\varphi(X) ; X \in A) \leq E \varphi(X), 
        \]
        where $A=\{X:P(|X|\geqslant a)\}$, $\varphi(X)=X^2$. So, we have
        \begin{align*}
            &i_{A}\,P(X \in A)=a^2\frac{b^2}{a^2}=b^2, \\
            &E(\varphi(X) ; X \in A)=a^2\frac{b^2}{a^2}=b^2, \\
            &E \varphi(X)=b^2. 
        \end{align*}
        So, it is sharp for such a r.v. $X$. 
        
        (ii), WLOG, let $X\sim N(0,1)$, then $EX=0$, $Var(X)=E(X^2)=1$. $A_a=\{X:P(|X|\geqslant a)\}$, then
        \[
            a^{2} P(|X| \geq a) / E X^{2}\leqslant x^2 P(|X| \geq a)=\int_{a}^\infty x^2 f(x)\der x, 
        \]
        where $f(\cdot)$ is pdf of $X$. So, 
        \[
            \lim_{a\to\infty}a^{2} P(|X| \geq a) / E X^{2}\longrightarrow 0, 
        \]
        And because $a^{2} P(|X| \geq a)<E(X^2)$, for any $a$, Chebyshev’s inequality is not sharp. 
    \end{proof}

    %%%%%%%%%%%%%%%%%%%%%%%%%%%%%%%%%%%%%%

    \begin{exercise}{1.6.9. Inclusion-exclusion formula.}
        Let $A_{1}, A_{2}, \ldots A_{n}$ be events and $A=\cup_{i=1}^{n} A_{i}$. Prove that $\mathbf{1}_{A}=1-\prod_{i=1}^{n}\left(1-\mathbf{1}_{A_{i}}\right)$. Expand out the right-hand side, then take expected value to conclude
        \begin{align*}
            P\left(\cup_{i=1}^{n} A_{i}\right)=& \sum_{i=1}^{n} P\left(A_{i}\right)-\sum_{i<j} P\left(A_{i} \cap A_{j}\right) \\
            &+\sum_{i<j<k} P\left(A_{i} \cap A_{j} \cap A_{k}\right)-\cdots+(-1)^{n-1} P\left(\cap_{i=1}^{n} A_{i}\right). 
        \end{align*}
    \end{exercise}

    \begin{proof}
        If $x\in A$, i.e. $x\in \cup_{i=1}^\infty A_i$. There must be at least one $i$, such that $x\in A_i$, $1-\mathbf{1}_{A_i}=1$. So, in this case, 
        \[
            \mathbf{1}_A=1=1-0=1-\prod_{i=1}^n(1-\mathbf{1}_{A_i}). 
        \] 
        If $x\not\in A$, the $\mathbf{1}_A=0$, and $\mathbf{1}_{A_i}=0$, for all $i$. Then
        \[
            \mathbf{1}_{A}=0=1-1=1-\prod_{i=1}^n(1-0)=1-\prod_{i=1}^n(1-\mathbf{1}_{A_i}). 
        \]
        For $\prod_{i=1}^n(1-\mathbf{1}_{A_i})$, we can expand it as
        \begin{align*}
            \mathbf{1}_A=&1-\prod_{i=1}^n(1-\mathbf{1}_{A_i})\\
            =&1-(1-\mathbf{1}_{A_1})(1-\mathbf{1}_{A_2})\cdots(1-\mathbf{1}_{A_n})\\
            =&(-1)^{0}\sum_{1\leqslant i\leqslant n}\mathbf{1}_{A_i}+(-1)^{1}\sum_{1\leqslant i<j\leqslant n}\mathbf{1}_{A_i}\mathbf{1}_{A_j}\\
            &+(-1)^{2}\sum_{1\leqslant i<j<k\leqslant n}\mathbf{1}_{A_i}\mathbf{1}_{A_j}\mathbf{1}_{A_k}-\cdots+(-1)^{n-1}\mathbf{1}_{A_1}\cdots\mathbf{1}_{A_n}\\
            =&\sum_{1\leqslant i\leqslant n}\mathbf{1}_{A_i}-\sum_{1\leqslant i<j\leqslant n}\mathbf{1}_{A_i}\mathbf{1}_{A_j}
            +\sum_{1\leqslant i<j<k\leqslant n}\mathbf{1}_{A_i}\mathbf{1}_{A_j}\mathbf{1}_{A_k}-\cdots+(-1)^{n-1}\mathbf{1}_{A_1}\cdots\mathbf{1}_{A_n}, 
        \end{align*}
        Take expectation for both sides, we can get
        \begin{align*}
            P(A)=P(\cup_{i=1}^nA_i)=&\sum_{1\leqslant i\leqslant n}P(A_i)-\sum_{1\leqslant i<j\leqslant n}P(A_i\cap A_j)\\
            &+\sum_{1\leqslant i<j<k\leqslant n}P(A_i\cap A_j\cap A_k)-\cdots+(-1)^{n-1}P(A_1\cap\cdots\cap A_n). 
        \end{align*}
        \vspace{-30pt}
    \end{proof}

    %%%%%%%%%%%%%%%%%%%%%%%%%%%%%%%%%%%%%%

    \begin{exercise}{1.6.10. Bonferroni inequalities.}
        Let $A_{1}, A_{2}, \ldots A_{n}$ be events and $A=\cup_{i=1}^{n} A_{i} .$ Show that $\mathbf{1}_{A} \leq \sum_{i=1}^{n} \mathbf{1}_{A_{i}}$, etc. and then take expected values to conclude
        \[
            P\left(\cup_{i=1}^{n} A_{i}\right) \leq \sum_{i=1}^{n} P\left(A_{i}\right), 
        \]
        \[
            P\left(\cup_{i=1}^{n} A_{i}\right) \geq \sum_{i=1}^{n} P\left(A_{i}\right)-\sum_{i<j} P\left(A_{i} \cap A_{j}\right), 
        \]
        \[
            P\left(\cup_{i=1}^{n} A_{i}\right) \leq \sum_{i=1}^{n} P\left(A_{i}\right)-\sum_{i<j} P\left(A_{i} \cap A_{j}\right)+\sum_{i<j<k} P\left(A_{i} \cap A_{j} \cap A_{k}\right). 
        \]
        In general, if we stop the inclusion-exclusion formula after an even (odd) number of sums, we get a(n) lower (upper) bound. 
    \end{exercise}
    \begin{proof}
        Becasue subadditivity, first inequality is apparent. For the second inequality, it equals to 
        \[
            \mathbf{1}_{A} \geqslant \sum_{1\leqslant i\leqslant n}^{n} \mathbf{1}_{A_{i}}-\sum_{1\leqslant i<j\leqslant n} \mathbf{1}_{A_{i}} \mathbf{1}_{A_{j}}, 
        \]
        Assume for $x\in A$, there are $m$ sets $A_i, \cdots, A_{i+m-1}$ satisfy $x\in A_i$, $m\geqslant2$. Then
        \[
            \sum_{1\leqslant i\leqslant n}^{n} \mathbf{1}_{A_{i}}-\sum_{1\leqslant i<j\leqslant n} \mathbf{1}_{A_{i}} \mathbf{1}_{A_{j}}
            =m-\binom{m}{2} \leqslant 1=\mathbf{1}_{A}. 
        \]
        Similarly, for the third inequality, we need to prove
        \[
            \mathbf{1}_{A} \leqslant \sum_{1\leqslant i\leqslant n}^{n} \mathbf{1}_{A_{i}}-\sum_{1\leqslant i<j\leqslant n} \mathbf{1}_{A_{i}} \mathbf{1}_{A_{j}}+\sum_{1\leqslant i<j<k\leqslant n} \mathbf{1}_{A_{i}} \mathbf{1}_{A_{j}}\mathbf{1}_{A_{k}}, 
        \]
        And if $m\geqslant3$, 
        \[
            \sum_{1\leqslant i\leqslant n}^{n} \mathbf{1}_{A_{i}}-\sum_{1\leqslant i<j\leqslant n} \mathbf{1}_{A_{i}} \mathbf{1}_{A_{j}}+\sum_{1\leqslant i<j<k\leqslant n} \mathbf{1}_{A_{i}} \mathbf{1}_{A_{j}}\mathbf{1}_{A_{k}}=m-\binom{m}{2}+\binom{m}{3}\geqslant1. 
        \]
        \vspace{-30pt}
    \end{proof}

    %%%%%%%%%%%%%%%%%%%%%%%%%%%%%%%%%%%%%%

    \begin{exercise}{1.6.11.}
        If $E|X|^{k}<\infty$, then for $0<j<k, E|X|^{j}<\infty$, and furthermore 
        \[
            E|X|^{j} \leq\left(E|X|^{k}\right)^{j / k}. 
        \]
    \end{exercise}

    \begin{proof}
        If $|X|^j\geqslant|X|^k$, then $|X|^j\leqslant|X|\leqslant1$. So, $E|X|^j\leqslant\infty$. If $|X|^j\leqslant|X|^k$, then because $E|X|^k\leqslant\infty$, $E|X|^j\leqslant\infty$. 
        
        For the inequality, let $\varphi(x)=x^{k/j}$. And because $\varphi$ is convex, we have
        \[
            E|X|^{k}=E\varphi\left(|X|^j\right)\geqslant\varphi\left(E|X|^j\right), 
        \]
        \[
            E|X|^{k}\geqslant\left(E|X|^j\right)^{k/j}, 
        \]
        \[
            \left(E|X|^{k}\right)^{j/k}\geqslant E|X|^j. 
        \]
        \vspace{-30pt}
    \end{proof}
\end{document}

